Refactoring leveled set interfaces

theories/Set/SetLevel.v
@@ -1,522 +1,539 @@
 From Coq Require Import MSets Lia.
 From DeBrLevel Require Import Level LevelInterface SetLevelInterface SetOTwL SetOTwLInterface.
 
-(** * Implementation -- Set of leveled elements *)
-
-(** ** Set implementation with minimal constraints *)
-Module IsLvlSetOTWL (T : IsLvlOTWL) <: (IsLvlSetOTWLInterface T).
-
-  Include SetOTWithLeibniz T.
-
-  (** *** Definition *)
-  Section definition.
-
-    Definition shift (lb : nat) (k : nat) (s : t) : t := map (T.shift lb k) s.
-
-    Definition valid (k : nat) (s : t) := (For_all (T.valid k) s).
-
-  End definition.
-
-  (** *** Valid *)
-  Section valid.
-
-    Variable lb : nat.
-    Variable v : elt.
-    Variable s s' : t.
-
-    Lemma valid_unfold : valid lb s <-> (For_all (T.valid lb) s).
-    Proof. unfold valid; split; auto. Qed.
-
-    Lemma valid_add_spec : valid lb (add v s) -> T.valid lb v /\ valid lb s.
-    Proof.
-      intros; unfold valid,For_all in *; split.
-      - apply H; apply add_spec; now left.
-      - intros. apply H; apply add_spec; now right.
-    Qed.
-
-    Lemma valid_empty_spec : valid lb empty.
-    Proof. intros; unfold valid,For_all; intros; inversion H. Qed.
-
-    Lemma valid_union_spec : valid lb (union s s') <-> valid lb s /\ valid lb s'.
-    Proof.
-      split; intros; unfold valid,For_all in *.
-      - split; intros; apply H; rewrite union_spec; auto.
-      - intros; destruct H; rewrite union_spec in *; destruct H0; auto.
-    Qed.
-
-    Lemma valid_singleton_spec : valid lb (singleton v) <-> T.valid lb v.
-    Proof.
-      split; intros; unfold valid,For_all in *.
-      - apply H; now rewrite singleton_spec.
-      - intros; rewrite singleton_spec in H0. apply T.eq_leibniz in H0; now subst.
-    Qed.
-
-    Lemma valid_in_spec : valid lb s -> In v s -> T.valid lb v.
-    Proof.
-      unfold valid,For_all in *; intros; now apply H.
-    Qed.
-
-  End valid.
-
-  (** *** Shift *)
-  Section shift.
-
-    Variable lb k : nat.
-    Variable v : elt.
-    Variable s : t.
-
-    #[local] Hint Resolve eq_equiv transpose_1 proper_1 : core.
+(** * Implementation - Set of leveled elements *)
 
 
-    Lemma shift_union_spec : forall s', 
-      shift lb k (union s s') = union (shift lb k s) (shift lb k s').
-    Proof. intros; unfold shift; now rewrite map_union_spec. Qed.
+Module IsLvlSet (T : IsLvlOTWL) (St : SetOTWithLeibnizInterface T) <: IsLvlSetInterface T St.
 
-    Lemma shift_Empty_spec : Empty s -> shift lb k s = empty.
-    Proof. intros; unfold shift; now apply map_Empty_spec. Qed.
+Import St.
 
-    Lemma shift_empty_spec : shift lb k empty = empty.
-    Proof. intros; unfold shift; now apply map_empty_spec. Qed.
+(** *** Definition *)
+Section definition.
 
-    Lemma shift_singleton_spec : shift lb k (singleton v) = singleton (T.shift lb k v).
-    Proof. intros; unfold shift; now apply map_singleton_spec. Qed.
+Definition t := t.
 
-    Lemma shift_add_notin_spec :
-      ~ In v s -> shift lb k (add v s) = add (T.shift lb k v) (shift lb k s).
-    Proof. intros; unfold shift; now apply map_add_notin_spec. Qed.
+Definition eq := eq.
+Definition eq_equiv := eq_equiv.
+Definition eq_dec := eq_dec.
+Definition eq_leibniz := eq_leibniz.
 
-    Lemma shift_add_in_spec :
-      In v s -> shift lb k (add v s) = (shift lb k s).
-    Proof. intros; unfold shift; now apply map_add_in_spec. Qed.
+Definition lt := lt.
+Definition lt_strorder := lt_strorder.
+Definition lt_compat := lt_compat.
 
-    Lemma shift_in_spec :
-      In v s <-> In (T.shift lb k v) (shift lb k s).
-    Proof.
-      unfold shift; induction s using set_induction.
-      - split; intro HIn; rewrite map_Empty_spec in *; auto; apply empty_is_empty_1 in H; 
-        apply eq_leibniz in H; subst; inversion HIn. 
-      - apply Add_inv in H0; subst; split; intro HIn; rewrite map_add_notin_spec in *; auto;
-        rewrite add_spec in *; destruct HIn.
-        -- apply T.eq_leibniz in H0; subst; left; reflexivity.
-        -- rewrite <- IHt0_1; now right. 
-        -- apply T.shift_eq_iff in H0; now left.
-        -- rewrite <- IHt0_1 in H0; now right.
-    Qed.
+Definition compare := compare.
+Definition compare_spec := compare_spec.
 
-    Lemma shift_add_spec :
-      shift lb k (add v s) = add (T.shift lb k v) (shift lb k s).
-    Proof.
-      intros; destruct (In_dec v s).
-      - rewrite shift_add_in_spec; auto. apply eq_leibniz; rewrite add_equal.
-        -- reflexivity.
-        -- now apply shift_in_spec.
-      - now  apply shift_add_notin_spec.
-    Qed.
+Definition shift (lb : nat) (k : nat) (s : t) : t := map (T.shift lb k) s.
 
-    Lemma shift_in_e_spec :
-      In v (shift lb k s) -> 
-      exists v', v = (T.shift lb k v') /\  In (T.shift lb k v') (shift lb k s).
-    Proof.
-      induction s using set_induction; intro HI; unfold shift in *.
-      - rewrite map_Empty_spec in HI; auto; inversion HI.
-      - apply Add_inv in H0; subst; rewrite map_add_notin_spec in HI; auto.
-        rewrite add_spec in *; destruct HI.
-        -- apply T.eq_leibniz in H0; rewrite H0; exists x; split; auto.
-          rewrite map_add_notin_spec; auto; apply add_spec; now left.
-        -- apply IHt0_1 in H0; destruct H0 as [r' [Heq HIn]]; subst.
-          exists r'; split; auto. rewrite map_add_notin_spec; auto; rewrite add_spec; now right.
-    Qed. 
+Definition valid (k : nat) (s : t) := (For_all (T.valid k) s).
 
-    Lemma shift_notin_spec : ~ In v s <-> ~ In (T.shift lb k v) (shift lb k s).
-    Proof.
-      intros; split; unfold not; intros; apply H.
-      - now rewrite <- shift_in_spec in H0.
-      - now rewrite <- shift_in_spec.
-    Qed.
+End definition.
 
-  End shift.
+(** *** Valid Property (part 1) *)
+Section valid.
 
-  (** *** Shift continued *)
-  Section shift_1.
+Variable lb : nat.
+Variable v : elt.
+Variable s s' : t.
 
-    Lemma shift_remove_spec : forall lb k v s,
-      shift lb k (remove v s) = remove (T.shift lb k v)(shift lb k s).
-    Proof.
-      intros lb k v s; revert lb k v;
-      induction s using set_induction; intros.
-      - symmetry; rewrite shift_Empty_spec; auto. 
-        apply empty_is_empty_1 in H. eapply Equal_remove in H; apply eq_leibniz in H; rewrite H.
-        apply eq_leibniz. split; intros.
-        -- rewrite remove_spec in H0; destruct H0. inversion H0.
-        -- apply shift_in_e_spec in H0.
-           destruct H0. destruct H0.
-           apply shift_in_spec in H1. rewrite remove_spec in H1; destruct H1; inversion H1.
-      
-      - apply Add_inv in H0; subst. apply eq_leibniz; split; intros.
-        -- apply shift_in_e_spec in H0. destruct H0; destruct H0.
-           apply shift_in_spec in H1. apply remove_spec in H1 as [H1 H1'].
-           rewrite remove_spec; split; subst.
-           + now apply shift_in_spec.
-           + intro; apply H1'. eapply T.shift_eq_iff; eauto.
-        -- apply remove_spec in H0 as [H0 H0']. rewrite shift_add_notin_spec in H0; auto.
-           apply add_spec in H0; destruct H0; subst.
-           + apply T.eq_leibniz in H0; subst; apply shift_in_spec. apply remove_spec; split.
-             ++ apply add_spec; now left.
-             ++ intro; apply H0'; subst; auto; apply T.eq_leibniz in H0;
-                subst; reflexivity.
-           + apply shift_in_e_spec in H0; destruct H0 as [y [Heq HIn]]; subst.
-             apply shift_in_spec. rewrite remove_spec; split.
-             ++ apply add_spec; right; now apply shift_in_spec in HIn.
-             ++ intro; apply H0'; apply T.eq_leibniz in H0; now subst.
-    Qed.
+Lemma valid_unfold : valid lb s <-> (For_all (T.valid lb) s).
+Proof. unfold valid; split; auto. Qed.
 
-    Lemma shift_eq_iff : forall lb k s s',
-      eq s s' <-> eq (shift lb k s) (shift lb k s').
-    Proof.
-      split.
-      - intro Heq; apply eq_leibniz in Heq; now subst.
-      - revert lb k s'; induction s using set_induction; intros lb k s'' Heq.
-        -- apply empty_is_empty_1 in H as H'.
-           apply eq_leibniz in H'; subst. eapply shift_Empty_spec in H; rewrite H in *.
-           symmetry in Heq. clear H. symmetry. revert lb k Heq.
-           induction s'' using set_induction; intros.
-           * apply empty_is_empty_1 in H; now rewrite H.
-           * apply Add_inv in H0; subst. rewrite shift_add_notin_spec in Heq; auto.
+Lemma valid_add_spec : valid lb (add v s) -> T.valid lb v /\ valid lb s.
+Proof.
+  intros; unfold valid,For_all in *; split.
+  - apply H; apply add_spec; now left.
+  - intros. apply H; apply add_spec; now right.
+Qed.
 
-             assert (eq (add (T.shift lb k x) (shift lb k s''1)) empty).
-             { now rewrite Heq. }
+Lemma valid_empty_spec : valid lb empty.
+Proof. intros; unfold valid,For_all; intros; inversion H. Qed.
 
-             apply empty_is_empty_2 in H0; unfold Empty in H0; exfalso.
-             apply (H0 (T.shift lb k x)). rewrite add_spec; now left.
-        -- apply Add_inv in H0; subst.
+Lemma valid_union_spec : valid lb (union s s') <-> valid lb s /\ valid lb s'.
+Proof.
+  split; intros; unfold valid,For_all in *.
+  - split; intros; apply H; rewrite union_spec; auto.
+  - intros; destruct H; rewrite union_spec in *; destruct H0; auto.
+Qed.
 
-           assert (forall s s' v, (add v s) = s' -> In v s').
-           { intros; subst; apply add_spec; now left. }
+Lemma valid_singleton_spec : valid lb (singleton v) <-> T.valid lb v.
+Proof.
+  split; intros; unfold valid,For_all in *.
+  - apply H; now rewrite singleton_spec.
+  - intros; rewrite singleton_spec in H0. apply T.eq_leibniz in H0; now subst.
+Qed.
 
-           rewrite shift_add_notin_spec in Heq; auto. apply eq_leibniz in Heq.
-           apply H0 in Heq as Heq'. apply add_remove in Heq' as Htmp.
-           apply eq_leibniz in Htmp. rewrite <- Htmp in Heq; clear Htmp.
-           rewrite <- shift_in_spec in Heq'. apply add_remove in Heq' as Htmp.
-           apply eq_leibniz in Htmp. rewrite <- Htmp; clear Htmp.
+Lemma valid_in_spec : valid lb s -> In v s -> T.valid lb v.
+Proof.
+  unfold valid,For_all in *; intros; now apply H.
+Qed.
 
-           assert (((add x s1) = (add x (remove x s''))) -> 
-                   (eq (add x s1) (add x (remove x s'')))) by (intro Hc; now rewrite Hc).
-           
-           apply H1; clear H1. f_equal. apply eq_leibniz; eapply IHs1.
-           rewrite <- add_eq_leibniz in Heq; eauto.
-           * rewrite Heq. now rewrite shift_remove_spec.
-           * now apply shift_notin_spec.
-           * rewrite remove_spec; intro. destruct H1; auto.
-             apply H2; reflexivity.
-    Qed.
+End valid.
 
-    Lemma shift_inter_spec : forall lb k s s', 
-      shift lb k (inter s s') = inter (shift lb k s) (shift lb k s').
-    Proof.
-      intros lb k s; induction s using set_induction; intros.
-      - apply empty_inter_1 with (s' := s') in H as H'.
-        unfold shift; rewrite map_Empty_spec; auto.
-        symmetry; rewrite map_Empty_spec; auto. apply eq_leibniz; split; intros.
-        -- rewrite inter_spec in H0; destruct H0; assumption.
-        -- inversion H0.
+(** *** Shift *)
+Section shift.
 
-      - apply Add_inv in H0; subst; unfold shift.
-        destruct (In_dec x s').
-        -- rewrite inter_in_add_spec; auto. rewrite map_add_notin_spec.
-          + symmetry; rewrite map_add_notin_spec; auto.
-            rewrite (shift_in_spec lb k) in i.
-            rewrite inter_in_add_spec; auto.
-            unfold shift in *. now rewrite IHs1.
-          + unfold not; intros; rewrite inter_spec in H0; destruct H0; contradiction.
+Variable lb k : nat.
+Variable v : elt.
+Variable s : t.
 
-        -- rewrite inter_notin_add_spec; auto. rewrite map_add_notin_spec; auto.
-          rewrite (shift_notin_spec lb k) in n.
-          rewrite inter_notin_add_spec; auto.
-          unfold shift in *. now rewrite IHs1.
-    Qed.
+#[local] Hint Resolve eq_equiv transpose_1 proper_1 : core.
 
-    Lemma shift_diff_spec : forall lb k s s',
-      shift lb k (diff s s') = (diff (shift lb k s) (shift lb k s')).
-    Proof.
-      intros lb k s; induction s using set_induction; intros.
+Lemma shift_union_spec : forall s', 
+  shift lb k (union s s') = union (shift lb k s) (shift lb k s').
+Proof. intros; unfold shift; now rewrite map_union_spec. Qed.
 
-      - apply eq_leibniz; split; unfold shift; intros.
-        -- apply empty_diff_1 with (s' := s') in H; rewrite map_Empty_spec in H0; auto.
-          inversion H0.
+Lemma shift_Empty_spec : Empty s -> shift lb k s = empty.
+Proof. intros; unfold shift; now apply map_Empty_spec. Qed.
 
-        -- rewrite diff_spec in H0; destruct H0; rewrite map_Empty_spec in H0; auto;
-          inversion H0.
-      
-      - apply eq_leibniz; split; intros.
-        
-        -- apply Add_inv in H0; subst; destruct (In_dec x s').
-          + rewrite diff_in_add_spec in H1; auto. rewrite IHs1 in H1.
-            rewrite diff_spec in *; destruct H1; split; auto.
-            unfold shift in *.
-            rewrite map_add_notin_spec; auto; rewrite add_spec; auto.
+Lemma shift_empty_spec : shift lb k empty = empty.
+Proof. intros; unfold shift; now apply map_empty_spec. Qed.
 
-          + rewrite diff_notin_add_spec in H1; auto. rewrite diff_spec in *.
-            replace (shift lb k (add x (diff s1 s')))
-            with ( add (T.shift lb k x) (shift lb k (diff s1 s'))) in H1.
-            ++ rewrite add_spec in H1; destruct H1.
-                * rewrite H0; split.
-                  ** unfold shift; rewrite map_add_notin_spec; auto.
-                    rewrite add_spec; left; reflexivity.
-                  ** now apply shift_notin_spec.
+Lemma shift_singleton_spec : shift lb k (singleton v) = singleton (T.shift lb k v).
+Proof. intros; unfold shift; now apply map_singleton_spec. Qed.
 
-                * rewrite IHs1 in *; rewrite diff_spec in H0; destruct H0.
-                  split; auto. unfold shift; rewrite map_add_notin_spec; auto.
-                  rewrite add_spec; right; apply H0.
+Lemma shift_add_notin_spec :
+  ~ In v s -> shift lb k (add v s) = add (T.shift lb k v) (shift lb k s).
+Proof. intros; unfold shift; now apply map_add_notin_spec. Qed.
 
-            ++ unfold shift; apply eq_leibniz; split; intros.
-                * rewrite add_spec in H0; destruct H0.
-                  ** rewrite H0; apply map_in_spec. rewrite add_spec; now left.
-                  ** unfold shift in *; rewrite IHs1 in H0; rewrite diff_spec in *.
-                    destruct H0. rewrite map_add_notin_spec.
-                    { rewrite add_spec; right; rewrite IHs1; rewrite diff_spec; auto. }
-                    { rewrite diff_notin_spec; auto. }
+Lemma shift_add_in_spec :
+  In v s -> shift lb k (add v s) = (shift lb k s).
+Proof. intros; unfold shift; now apply map_add_in_spec. Qed.
 
-                * rewrite map_add_notin_spec in H0.
-                  ** rewrite add_spec in *; auto.
-                  ** rewrite diff_notin_spec; auto.
+Lemma shift_in_spec :
+  In v s <-> In (T.shift lb k v) (shift lb k s).
+Proof.
+  unfold shift; induction s using set_induction.
+  - split; intro HIn; rewrite map_Empty_spec in *; auto; apply empty_is_empty_1 in H; 
+    apply eq_leibniz in H; subst; inversion HIn. 
+  - apply Add_inv in H0; subst; split; intro HIn; rewrite map_add_notin_spec in *; auto;
+    rewrite add_spec in *; destruct HIn.
+    -- apply T.eq_leibniz in H0; subst; left; reflexivity.
+    -- rewrite <- IHt0_1; now right. 
+    -- apply T.shift_eq_iff in H0; now left.
+    -- rewrite <- IHt0_1 in H0; now right.
+Qed.
 
-        -- apply Add_inv in H0; subst; destruct (In_dec x s').
-          + rewrite diff_in_add_spec; auto; rewrite IHs1. rewrite diff_spec in *; 
-            destruct H1; split; auto.
-            unfold shift in *. rewrite map_add_notin_spec in H0; auto.
-            rewrite add_spec in H0; destruct H0; auto; rewrite H0 in *.
-            unfold not in *; exfalso; apply H1; now apply map_in_spec.
-          + rewrite diff_notin_add_spec; auto. rewrite diff_spec in H1. 
-            destruct H1; unfold shift in *. rewrite map_add_notin_spec in H0; auto.
-            rewrite add_spec in H0; destruct H0.
-            ++ rewrite H0 in *; rewrite map_add_notin_spec.
-                * rewrite add_spec; left; reflexivity.
-                * apply diff_notin_spec; auto.
-            ++ rewrite map_add_notin_spec.
-                * rewrite add_spec; right; rewrite IHs1; rewrite diff_spec; split; auto.
-                * apply diff_notin_spec; auto.
-    Qed.
+Lemma shift_add_spec :
+  shift lb k (add v s) = add (T.shift lb k v) (shift lb k s).
+Proof.
+  intros; destruct (In_dec v s).
+  - rewrite shift_add_in_spec; auto. apply eq_leibniz; rewrite add_equal.
+    -- reflexivity.
+    -- now apply shift_in_spec.
+  - now  apply shift_add_notin_spec.
+Qed.
+
+Lemma shift_in_e_spec :
+  In v (shift lb k s) -> 
+  exists v', v = (T.shift lb k v') /\  In (T.shift lb k v') (shift lb k s).
+Proof.
+  induction s using set_induction; intro HI; unfold shift in *.
+  - rewrite map_Empty_spec in HI; auto; inversion HI.
+  - apply Add_inv in H0; subst; rewrite map_add_notin_spec in HI; auto.
+    rewrite add_spec in *; destruct HI.
+    -- apply T.eq_leibniz in H0; rewrite H0; exists x; split; auto.
+      rewrite map_add_notin_spec; auto; apply add_spec; now left.
+    -- apply IHt0_1 in H0; destruct H0 as [r' [Heq HIn]]; subst.
+      exists r'; split; auto. rewrite map_add_notin_spec; auto; rewrite add_spec; now right.
+Qed. 
+
+Lemma shift_notin_spec : ~ In v s <-> ~ In (T.shift lb k v) (shift lb k s).
+Proof.
+  intros; split; unfold not; intros; apply H.
+  - now rewrite <- shift_in_spec in H0.
+  - now rewrite <- shift_in_spec.
+Qed.
+
+End shift.
+
+Lemma shift_remove_spec : forall lb k v s,
+  shift lb k (remove v s) = remove (T.shift lb k v)(shift lb k s).
+Proof.
+  intros lb k v s; revert lb k v;
+  induction s using set_induction; intros.
+  - symmetry; rewrite shift_Empty_spec; auto. 
+    apply empty_is_empty_1 in H. eapply Equal_remove in H; apply eq_leibniz in H; rewrite H.
+    apply eq_leibniz. split; intros.
+    -- rewrite remove_spec in H0; destruct H0. inversion H0.
+    -- apply shift_in_e_spec in H0.
+        destruct H0. destruct H0.
+        apply shift_in_spec in H1. rewrite remove_spec in H1; destruct H1; inversion H1.
   
-    Lemma shift_zero_refl : forall lb s,
-      eq (shift lb 0 s) s.
-    Proof.
-      unfold shift; intros. induction s using set_induction.
-      - apply empty_is_empty_1 in H; apply eq_leibniz in H; subst.  
-        now rewrite map_empty_spec.
-      - apply Add_inv in H0; subst; rewrite map_add_notin_spec; auto.
-        apply eq_leibniz in IHs1; rewrite IHs1; rewrite T.shift_zero_refl; reflexivity.
-    Qed.
+  - apply Add_inv in H0; subst. apply eq_leibniz; split; intros.
+    -- apply shift_in_e_spec in H0. destruct H0; destruct H0.
+        apply shift_in_spec in H1. apply remove_spec in H1 as [H1 H1'].
+        rewrite remove_spec; split; subst.
+        + now apply shift_in_spec.
+        + intro; apply H1'. eapply T.shift_eq_iff; eauto.
+    -- apply remove_spec in H0 as [H0 H0']. rewrite shift_add_notin_spec in H0; auto.
+        apply add_spec in H0; destruct H0; subst.
+        + apply T.eq_leibniz in H0; subst; apply shift_in_spec. apply remove_spec; split.
+          ++ apply add_spec; now left.
+          ++ intro; apply H0'; subst; auto; apply T.eq_leibniz in H0;
+            subst; reflexivity.
+        + apply shift_in_e_spec in H0; destruct H0 as [y [Heq HIn]]; subst.
+          apply shift_in_spec. rewrite remove_spec; split.
+          ++ apply add_spec; right; now apply shift_in_spec in HIn.
+          ++ intro; apply H0'; apply T.eq_leibniz in H0; now subst.
+Qed.
 
-    Lemma shift_eq : Proper (Logic.eq ==> Logic.eq ==> eq ==> eq) shift.
-    Proof. 
-      red; red; red; red; intros; subst. apply eq_leibniz in H1; now subst.
-    Qed.
+Lemma shift_eq_iff : forall lb k s s',
+  eq s s' <-> eq (shift lb k s) (shift lb k s').
+Proof.
+  split.
+  - intro Heq; apply eq_leibniz in Heq; now subst.
+  - revert lb k s'; induction s using set_induction; intros lb k s'' Heq.
+    -- apply empty_is_empty_1 in H as H'.
+        apply eq_leibniz in H'; subst. eapply shift_Empty_spec in H; rewrite H in *.
+        symmetry in Heq. clear H. symmetry. revert lb k Heq.
+        induction s'' using set_induction; intros.
+        * apply empty_is_empty_1 in H; now rewrite H.
+        * apply Add_inv in H0; subst. rewrite shift_add_notin_spec in Heq; auto.
 
-    Lemma shift_trans : forall lb k k' s,
-      eq (shift lb k (shift lb k' s)) (shift lb (k + k') s).
-    Proof.
-      intros lb k k' s; induction s using set_induction; unfold shift.
-      - repeat rewrite map_Empty_spec; auto; reflexivity.
-      - apply Add_inv in H0; subst. repeat rewrite map_add_notin_spec; auto.
-        -- split; intros HI; rewrite add_spec in *; destruct HI.
-          + left; rewrite H0; now rewrite T.shift_trans.
-          + right; unfold shift in IHs1. now rewrite <- IHs1.
-          + left; rewrite H0; now rewrite T.shift_trans.
-          + right. unfold shift in IHs1. now rewrite IHs1.
-        -- rewrite shift_notin_spec in H; eauto.
-    Qed.
+          assert (eq (add (T.shift lb k x) (shift lb k s''1)) empty).
+          { now rewrite Heq. }
 
-    Lemma shift_permute : forall lb k k' s,
-      eq (shift lb k (shift lb k' s)) (shift lb k' (shift lb k s)).
-    Proof.
-      intros lb k k' s; induction s using set_induction; unfold shift.
-      - repeat rewrite map_Empty_spec; auto; reflexivity.
-      - apply Add_inv in H0; subst; repeat rewrite map_add_notin_spec; auto;
-        try (rewrite shift_notin_spec in H; now eauto).
-        split; intros; rewrite add_spec in *; destruct H0.
-        -- left; rewrite H0; apply T.shift_permute.
-        -- right; unfold shift in *; now rewrite <- IHs1.
-        -- left; rewrite H0; apply T.shift_permute.
-        -- right; unfold shift in *; now rewrite IHs1.
-    Qed.
+          apply empty_is_empty_2 in H0; unfold Empty in H0; exfalso.
+          apply (H0 (T.shift lb k x)). rewrite add_spec; now left.
+    -- apply Add_inv in H0; subst.
 
-    Lemma shift_unfold : forall lb k k' t,
-      eq (shift lb (k + k') t) (shift (lb + k) k' (shift lb k t)). 
-    Proof.
-      intros lb k k' t; induction t using set_induction.
-      - unfold shift; repeat rewrite map_Empty_spec; auto. reflexivity.
-      - apply Add_inv in H0; subst. repeat rewrite shift_add_notin_spec; eauto.
-        -- rewrite T.shift_unfold; rewrite IHt1; reflexivity.
-        -- now apply shift_notin_spec.
-    Qed.
+        assert (forall s s' v, (add v s) = s' -> In v s').
+        { intros; subst; apply add_spec; now left. }
 
-    Lemma shift_unfold_1 : forall k k' k'' t,
-      k <= k' -> k' <= k'' -> 
-      eq (shift k' (k'' - k') (shift k  (k' - k) t)) (shift k (k'' - k) t).
-    Proof.
-      intros k k' k'' t; induction t using set_induction; intros.
-      - unfold shift; repeat rewrite map_Empty_spec; auto. reflexivity.
-      - apply Add_inv in H0; subst. repeat rewrite shift_add_notin_spec; eauto.
-        -- rewrite T.shift_unfold_1; auto; rewrite IHt1; auto; reflexivity.
-        -- now apply shift_notin_spec.
-    Qed.
+        rewrite shift_add_notin_spec in Heq; auto. apply eq_leibniz in Heq.
+        apply H0 in Heq as Heq'. apply add_remove in Heq' as Htmp.
+        apply eq_leibniz in Htmp. rewrite <- Htmp in Heq; clear Htmp.
+        rewrite <- shift_in_spec in Heq'. apply add_remove in Heq' as Htmp.
+        apply eq_leibniz in Htmp. rewrite <- Htmp; clear Htmp.
 
-  End shift_1.
+        assert (((add x s1) = (add x (remove x s''))) -> 
+                (eq (add x s1) (add x (remove x s'')))) by (intro Hc; now rewrite Hc).
+        
+        apply H1; clear H1. f_equal. apply eq_leibniz; eapply IHs1.
+        rewrite <- add_eq_leibniz in Heq; eauto.
+        * rewrite Heq. now rewrite shift_remove_spec.
+        * now apply shift_notin_spec.
+        * rewrite remove_spec; intro. destruct H1; auto.
+          apply H2; reflexivity.
+Qed.
 
-  (** *** Valid continued *)
-  Section valid_1.
+Lemma shift_inter_spec : forall lb k s s', 
+  shift lb k (inter s s') = inter (shift lb k s) (shift lb k s').
+Proof.
+  intros lb k s; induction s using set_induction; intros.
+  - apply empty_inter_1 with (s' := s') in H as H'.
+    unfold shift; rewrite map_Empty_spec; auto.
+    symmetry; rewrite map_Empty_spec; auto. apply eq_leibniz; split; intros.
+    -- rewrite inter_spec in H0; destruct H0; assumption.
+    -- inversion H0.
 
-    Lemma valid_eq : Proper (Logic.eq ==> eq ==> iff) valid.
-    Proof.
-      repeat red; intros; apply eq_leibniz in H0; subst; split; auto.
-    Qed.
+  - apply Add_inv in H0; subst; unfold shift.
+    destruct (In_dec x s').
+    -- rewrite inter_in_add_spec; auto. rewrite map_add_notin_spec.
+      + symmetry; rewrite map_add_notin_spec; auto.
+        rewrite (shift_in_spec lb k) in i.
+        rewrite inter_in_add_spec; auto.
+        unfold shift in *. now rewrite IHs1.
+      + unfold not; intros; rewrite inter_spec in H0; destruct H0; contradiction.
 
-    Lemma valid_weakening: forall k k' s,
-      (k <= k') -> valid k s -> valid k' s.
-    Proof. 
-      intros; unfold valid,For_all in *; intros; apply H0 in H1. 
-      eapply T.valid_weakening; eauto.
-    Qed.
+    -- rewrite inter_notin_add_spec; auto. rewrite map_add_notin_spec; auto.
+      rewrite (shift_notin_spec lb k) in n.
+      rewrite inter_notin_add_spec; auto.
+      unfold shift in *. now rewrite IHs1.
+Qed.
 
-    Theorem shift_preserves_valid_1 : forall lb k k' s,
-      valid k s -> valid (k + k') (shift lb k' s).
-    Proof.
-      unfold valid,For_all in *; intros.
-      apply shift_in_e_spec in H0; destruct H0 as [y [Heq HIn]]; subst.
-      apply T.shift_preserves_valid_1; apply H; now rewrite <- shift_in_spec in HIn.
-    Qed.
+Lemma shift_diff_spec : forall lb k s s',
+  shift lb k (diff s s') = (diff (shift lb k s) (shift lb k s')).
+Proof.
+  intros lb k s; induction s using set_induction; intros.
 
-    Theorem shift_preserves_valid : forall k k' s,
-      valid k s -> valid (k + k') (shift k k' s).
-    Proof. intros; now apply shift_preserves_valid_1. Qed.
+  - apply eq_leibniz; split; unfold shift; intros.
+    -- apply empty_diff_1 with (s' := s') in H; rewrite map_Empty_spec in H0; auto.
+      inversion H0.
 
-    Lemma shift_preserves_valid_zero : forall k t, valid k t -> valid k (shift k 0 t).
-    Proof. intros; replace k with (k + 0); try lia; now apply shift_preserves_valid_1. Qed.
+    -- rewrite diff_spec in H0; destruct H0; rewrite map_Empty_spec in H0; auto;
+      inversion H0.
+  
+  - apply eq_leibniz; split; intros.
+    
+    -- apply Add_inv in H0; subst; destruct (In_dec x s').
+      + rewrite diff_in_add_spec in H1; auto. rewrite IHs1 in H1.
+        rewrite diff_spec in *; destruct H1; split; auto.
+        unfold shift in *.
+        rewrite map_add_notin_spec; auto; rewrite add_spec; auto.
 
-    Lemma shift_preserves_valid_gen : forall lb lb' k k' t,
-      k <= k' -> lb <= lb' -> k <= lb -> k' <= lb' -> k' - k = lb' - lb -> 
-      valid lb t -> valid lb' (shift k (k' - k) t).
-    Proof.
-      unfold valid,For_all in *; intros. apply shift_in_e_spec in H5. 
-      destruct H5 as [y [Heq HIn]]; subst.
-      apply T.shift_preserves_valid_gen with (lb := lb); auto.
-      apply H4. now rewrite <- shift_in_spec in HIn.
-    Qed.
+      + rewrite diff_notin_add_spec in H1; auto. rewrite diff_spec in *.
+        replace (shift lb k (add x (diff s1 s')))
+        with ( add (T.shift lb k x) (shift lb k (diff s1 s'))) in H1.
+        ++ rewrite add_spec in H1; destruct H1.
+            * rewrite H0; split.
+              ** unfold shift; rewrite map_add_notin_spec; auto.
+                rewrite add_spec; left; reflexivity.
+              ** now apply shift_notin_spec.
 
-    Lemma shift_preserves_valid_2 : forall lb lb' t,
-      lb <= lb' -> valid lb t -> 
-      valid lb' (shift lb (lb' - lb) t).
-    Proof. intros. eapply shift_preserves_valid_gen; eauto. Qed.
+            * rewrite IHs1 in *; rewrite diff_spec in H0; destruct H0.
+              split; auto. unfold shift; rewrite map_add_notin_spec; auto.
+              rewrite add_spec; right; apply H0.
+
+        ++ unfold shift; apply eq_leibniz; split; intros.
+            * rewrite add_spec in H0; destruct H0.
+              ** rewrite H0; apply map_in_spec. rewrite add_spec; now left.
+              ** unfold shift in *; rewrite IHs1 in H0; rewrite diff_spec in *.
+                destruct H0. rewrite map_add_notin_spec.
+                { rewrite add_spec; right; rewrite IHs1; rewrite diff_spec; auto. }
+                { rewrite diff_notin_spec; auto. }
+
+            * rewrite map_add_notin_spec in H0.
+              ** rewrite add_spec in *; auto.
+              ** rewrite diff_notin_spec; auto.
+
+    -- apply Add_inv in H0; subst; destruct (In_dec x s').
+      + rewrite diff_in_add_spec; auto; rewrite IHs1. rewrite diff_spec in *; 
+        destruct H1; split; auto.
+        unfold shift in *. rewrite map_add_notin_spec in H0; auto.
+        rewrite add_spec in H0; destruct H0; auto; rewrite H0 in *.
+        unfold not in *; exfalso; apply H1; now apply map_in_spec.
+      + rewrite diff_notin_add_spec; auto. rewrite diff_spec in H1. 
+        destruct H1; unfold shift in *. rewrite map_add_notin_spec in H0; auto.
+        rewrite add_spec in H0; destruct H0.
+        ++ rewrite H0 in *; rewrite map_add_notin_spec.
+            * rewrite add_spec; left; reflexivity.
+            * apply diff_notin_spec; auto.
+        ++ rewrite map_add_notin_spec.
+            * rewrite add_spec; right; rewrite IHs1; rewrite diff_spec; split; auto.
+            * apply diff_notin_spec; auto.
+Qed.
+
+Lemma shift_zero_refl : forall lb s,
+  eq (shift lb 0 s) s.
+Proof.
+  unfold shift; intros. induction s using set_induction.
+  - apply empty_is_empty_1 in H; apply eq_leibniz in H; subst.  
+    now rewrite map_empty_spec.
+  - apply Add_inv in H0; subst; rewrite map_add_notin_spec; auto.
+    apply eq_leibniz in IHs1; rewrite IHs1; rewrite T.shift_zero_refl; reflexivity.
+Qed.
+
+Lemma shift_eq : Proper (Logic.eq ==> Logic.eq ==> eq ==> eq) shift.
+Proof. 
+  red; red; red; red; intros; subst. apply eq_leibniz in H1; now subst.
+Qed.
+
+Lemma shift_trans : forall lb k k' s,
+  eq (shift lb k (shift lb k' s)) (shift lb (k + k') s).
+Proof.
+  intros lb k k' s; induction s using set_induction; unfold shift.
+  - repeat rewrite map_Empty_spec; auto; reflexivity.
+  - apply Add_inv in H0; subst. repeat rewrite map_add_notin_spec; auto.
+    -- split; intros HI; rewrite add_spec in *; destruct HI.
+      + left; rewrite H0; now rewrite T.shift_trans.
+      + right; unfold shift in IHs1. now rewrite <- IHs1.
+      + left; rewrite H0; now rewrite T.shift_trans.
+      + right. unfold shift in IHs1. now rewrite IHs1.
+    -- rewrite shift_notin_spec in H; eauto.
+Qed.
+
+Lemma shift_permute : forall lb k k' s,
+  eq (shift lb k (shift lb k' s)) (shift lb k' (shift lb k s)).
+Proof.
+  intros lb k k' s; induction s using set_induction; unfold shift.
+  - repeat rewrite map_Empty_spec; auto; reflexivity.
+  - apply Add_inv in H0; subst; repeat rewrite map_add_notin_spec; auto;
+    try (rewrite shift_notin_spec in H; now eauto).
+    split; intros; rewrite add_spec in *; destruct H0.
+    -- left; rewrite H0; apply T.shift_permute.
+    -- right; unfold shift in *; now rewrite <- IHs1.
+    -- left; rewrite H0; apply T.shift_permute.
+    -- right; unfold shift in *; now rewrite IHs1.
+Qed.
+
+Lemma shift_unfold : forall lb k k' t,
+  eq (shift lb (k + k') t) (shift (lb + k) k' (shift lb k t)). 
+Proof.
+  intros lb k k' t; induction t using set_induction.
+  - unfold shift; repeat rewrite map_Empty_spec; auto. reflexivity.
+  - apply Add_inv in H0; subst. repeat rewrite shift_add_notin_spec; eauto.
+    -- rewrite T.shift_unfold; rewrite IHt1; reflexivity.
+    -- now apply shift_notin_spec.
+Qed.
+
+Lemma shift_unfold_1 : forall k k' k'' t,
+  k <= k' -> k' <= k'' -> 
+  eq (shift k' (k'' - k') (shift k  (k' - k) t)) (shift k (k'' - k) t).
+Proof.
+  intros k k' k'' t; induction t using set_induction; intros.
+  - unfold shift; repeat rewrite map_Empty_spec; auto. reflexivity.
+  - apply Add_inv in H0; subst. repeat rewrite shift_add_notin_spec; eauto.
+    -- rewrite T.shift_unfold_1; auto; rewrite IHt1; auto; reflexivity.
+    -- now apply shift_notin_spec.
+Qed.
+
+(** *** Valid property (part 2) *)
+
+#[export]
+Instance valid_eq : Proper (Logic.eq ==> eq ==> iff) valid.
+Proof.
+  repeat red; intros; apply eq_leibniz in H0; subst; split; auto.
+Qed.
+
+Lemma valid_weakening: forall k k' s,
+  (k <= k') -> valid k s -> valid k' s.
+Proof. 
+  intros; unfold valid,For_all in *; intros; apply H0 in H1. 
+  eapply T.valid_weakening; eauto.
+Qed.
+
+Theorem shift_preserves_valid_1 : forall lb k k' s,
+  valid k s -> valid (k + k') (shift lb k' s).
+Proof.
+  unfold valid,For_all in *; intros.
+  apply shift_in_e_spec in H0; destruct H0 as [y [Heq HIn]]; subst.
+  apply T.shift_preserves_valid_1; apply H; now rewrite <- shift_in_spec in HIn.
+Qed.
+
+Theorem shift_preserves_valid : forall k k' s,
+  valid k s -> valid (k + k') (shift k k' s).
+Proof. intros; now apply shift_preserves_valid_1. Qed.
+
+Lemma shift_preserves_valid_zero : forall k t, valid k t -> valid k (shift k 0 t).
+Proof. intros; replace k with (k + 0); try lia; now apply shift_preserves_valid_1. Qed.
+
+Lemma shift_preserves_valid_gen : forall lb lb' k k' t,
+  k <= k' -> lb <= lb' -> k <= lb -> k' <= lb' -> k' - k = lb' - lb -> 
+  valid lb t -> valid lb' (shift k (k' - k) t).
+Proof.
+  unfold valid,For_all in *; intros. apply shift_in_e_spec in H5. 
+  destruct H5 as [y [Heq HIn]]; subst.
+  apply T.shift_preserves_valid_gen with (lb := lb); auto.
+  apply H4. now rewrite <- shift_in_spec in HIn.
+Qed.
+
+Lemma shift_preserves_valid_2 : forall lb lb' t,
+  lb <= lb' -> valid lb t -> 
+  valid lb' (shift lb (lb' - lb) t).
+Proof. intros. eapply shift_preserves_valid_gen; eauto. Qed.
+
+End IsLvlSet.
 
 
-  End valid_1.
+Module IsBdlLvlSet (T : IsBdlLvlOTWL) (Se : SetOTWithLeibnizInterface T) <: IsBdlLvlOTWL.
 
-End IsLvlSetOTWL.
+Include IsLvlSet T Se.
+Import Se.
 
-(** ** Set implementation with fully constrained *)
-Module IsBdlLvlSetOTWL (T : IsBdlLvlOTWL) 
-                                            <: IsBdlLvlSetOTWLInterface T.
+Lemma shift_valid_refl : forall lb k s,
+  valid lb s -> eq (shift lb k s) s.
+Proof.
+  intros lb k s; induction s using set_induction; intros.
+  - apply empty_is_empty_1 in H; apply eq_leibniz in H; subst.
+    now rewrite shift_empty_spec.
+  
+  - apply Add_inv in H0; subst.
+    rewrite shift_add_notin_spec; try assumption.
+    apply valid_add_spec in H1; destruct H1; f_equal.
+    rewrite T.shift_valid_refl; auto.
+    apply IHs1 in H1; now rewrite H1.
+Qed.
 
-  Include IsLvlSetOTWL T.
+End IsBdlLvlSet.
 
-    Lemma shift_valid_refl : forall lb k s,
-      valid lb s -> eq (shift lb k s) s.
-    Proof.
-      intros lb k s; induction s using set_induction; intros.
-      - apply empty_is_empty_1 in H; apply eq_leibniz in H; subst.
-        now rewrite shift_empty_spec.
-      
-      - apply Add_inv in H0; subst.
-        rewrite shift_add_notin_spec; try assumption.
-        apply valid_add_spec in H1; destruct H1; f_equal.
-        rewrite T.shift_valid_refl; auto.
-        apply IHs1 in H1; now rewrite H1.
-    Qed.
 
-End IsBdlLvlSetOTWL.
+Module IsLvlFullSet (T : IsLvlFullOTWL) (Se : SetOTWithLeibnizInterface T)
+                                            <: IsLvlFullSetInterface T Se.
 
-(** ** Set implementation with minimal constraints with [validb] *)
-Module IsLvlFullSetOTWL (T : IsLvlFullOTWL) 
-                                            <: IsLvlFullSetOTWLInterface T.
+Include IsLvlSet T Se.
+Import Se.
 
-  Include IsLvlSetOTWL T.
+(** ** Definition *)
+Definition validb (k : nat) (s : t) := (for_all (fun v => T.validb k v) s).
 
-  (** *** Definition *)
-  Section definition.
+(** ** Valid *)
+#[export]
+Instance proper_valid : Proper (Logic.eq ==> T.eq ==> Logic.eq) T.validb.
+Proof. repeat red; intros; subst. apply T.eq_leibniz in H0; now subst. Qed.
 
-    Definition validb (k : nat) (s : t) := (for_all (fun v => T.validb k v) s).
+Lemma validb_valid : forall k t, validb k t = true <-> valid k t. 
+Proof.
+  unfold valid,validb; split; intros; rewrite for_all_spec in *; unfold For_all in *;
+  try (repeat red; intros; now subst); auto.
+  - intros; rewrite <- T.validb_valid; auto.
+  - repeat red; intros; subst. apply T.eq_leibniz in H0; now subst.
+  - intros; rewrite T.validb_valid; auto.
+  - repeat red; intros; subst. apply T.eq_leibniz in H0; now subst.
+Qed.
 
-  End definition.
+Lemma validb_nvalid : forall k t, validb k t = false <-> ~ valid k t.
+Proof.
+  intros; rewrite <- not_true_iff_false; split; intros; intro.
+  - apply H; now rewrite validb_valid. 
+  - apply H; now rewrite <- validb_valid.
+Qed.
 
-  (** *** Valid *)
-  Section valid.
+#[export]
+Instance validb_eq : Proper (Logic.eq ==> eq ==> Logic.eq) validb.
+Proof. repeat red; intros; subst; apply eq_leibniz in H0; now subst. Qed.
 
-    Fact proper_valid : forall k, Proper (T.eq ==> Logic.eq) (fun (v : elt) => T.validb k v).
-    Proof. repeat red; intros; subst; apply T.eq_leibniz in H; now subst. Qed.
+End IsLvlFullSet.
 
-    #[local] Hint Resolve proper_valid : core.
 
-    Lemma validb_valid : forall k t, validb k t = true <-> valid k t. 
-    Proof.
-      unfold valid,validb; split; intros; rewrite for_all_spec in *; unfold For_all in *;
-      try (repeat red; intros; now subst); auto.
-      - intros; rewrite <- T.validb_valid; auto.
-      - intros; rewrite T.validb_valid; auto.
-    Qed.
+Module IsBdlLvlFullSet (T : IsBdlLvlFullOTWL) (Se : SetOTWithLeibnizInterface T)
+                                                     <: IsBdlLvlFullSetInterface T Se.
 
-    Lemma validb_nvalid : forall k t, validb k t = false <-> ~ valid k t.
-    Proof.
-      intros; rewrite <- not_true_iff_false; split; intros; intro.
-      - apply H; now rewrite validb_valid. 
-      - apply H; now rewrite <- validb_valid.
-    Qed.
+Include IsLvlFullSet T Se.
+Import Se.
 
-    Lemma validb_eq : Proper (Logic.eq ==> eq ==> Logic.eq) validb.
-    Proof. repeat red; intros; subst; apply eq_leibniz in H0; now subst. Qed.
+Lemma shift_valid_refl : forall lb k s,
+  valid lb s -> eq (shift lb k s) s.
+Proof.
+  intros lb k s; induction s using set_induction; intros.
+  - apply empty_is_empty_1 in H; apply eq_leibniz in H; subst.
+    now rewrite shift_empty_spec.
+  
+  - apply Add_inv in H0; subst.
+    rewrite shift_add_notin_spec; try assumption.
+    apply valid_add_spec in H1; destruct H1; f_equal.
+    rewrite T.shift_valid_refl; auto.
+    apply IHs1 in H1; now rewrite H1.
+Qed.
 
-  End valid.
+End IsBdlLvlFullSet.
 
-End IsLvlFullSetOTWL.
+(** ** Make - Leveled Set *)
 
-(** ** Set implementation with fully constrained with [validb] *)
-Module IsBdlLvlFullSetOTWL (T : IsBdlLvlFullOTWL) 
-                                                <: IsBdlLvlFullSetOTWLInterface T.
+Module MakeIsLvlSet (T : IsLvlOTWL) <: IsLvlOTWL.
 
-  Include IsBdlLvlSetOTWL T.
+  Module St := SetOTWithLeibniz T.
+  Include IsLvlSet T St.
+  Import St.
 
-  (** *** Definition *)
-  Section definition.
+End MakeIsLvlSet.
 
-    Definition validb (k : nat) (s : t) := (for_all (fun v => T.validb k v) s).
 
-  End definition.
+Module MakeIsBdlLvlSet (T : IsBdlLvlOTWL) <: IsBdlLvlOTWL.
 
-  (** *** Valid *)
-  Section valid.
+  Module St := SetOTWithLeibniz T.
+  Include IsBdlLvlSet T St.
+  Import St.
 
-    Fact proper_valid : forall k, Proper (T.eq ==> Logic.eq) (fun (v : elt) => T.validb k v).
-    Proof. repeat red; intros; subst; apply T.eq_leibniz in H; now subst. Qed.
+End MakeIsBdlLvlSet.
 
-    #[local] Hint Resolve proper_valid : core.
 
-    Lemma validb_valid : forall k t, validb k t = true <-> valid k t. 
-    Proof.
-      unfold valid,validb; split; intros; rewrite for_all_spec in *; unfold For_all in *;
-      try (repeat red; intros; now subst); auto.
-      - intros; rewrite <- T.validb_valid; auto.
-      - intros; rewrite T.validb_valid; auto.
-    Qed.
+Module MakeIsLvlFullSet (T : IsLvlFullOTWL) <: IsLvlFullOTWL.
 
-    Lemma validb_nvalid : forall k t, validb k t = false <-> ~ valid k t.
-    Proof.
-      intros; rewrite <- not_true_iff_false; split; intros; intro.
-      - apply H; now rewrite validb_valid. 
-      - apply H; now rewrite <- validb_valid.
-    Qed.
+  Module St := SetOTWithLeibniz T.
+  Include IsLvlFullSet T St.
+  Import St.
 
-    Lemma validb_eq : Proper (Logic.eq ==> eq ==> Logic.eq) validb.
-    Proof. repeat red; intros; subst; apply eq_leibniz in H0; now subst. Qed.
+End MakeIsLvlFullSet.
 
-  End valid.
 
-End IsBdlLvlFullSetOTWL.
+Module MakeIsBdlLvlFullSet (T : IsBdlLvlFullOTWL) <: IsBdlLvlFullOTWL.
+
+  Module St := SetOTWithLeibniz T.
+  Include IsBdlLvlFullSet T St.
+  Import St.
+
+End MakeIsBdlLvlFullSet.
