theories/Set/SetLevelInterface.v
@@ -1,35 +1,45 @@
 From Coq Require Import MSets.
-From DeBrLevel Require Import Level LevelInterface SetOTwLInterface SetOTwL.
+From DeBrLevel Require Import LevelInterface SetOTwLInterface SetOTwL.
 
-(** * Interfaces -- Set Level
+(** * Interface - Leveled Set
 
-  Based on the overlay [SetOTwL] we defined interfaces for sets with [shift] and [valid].
+  Based on [SetOTwL], we define interfaces for sets with leveled elements. In addition to
+  properties on [shift] and [valid], we ask the user to satisfy several interaction properties
+  between them and classical set operators such as ∈,∪, etc.
+
+  [shift] is directly applied on elements of the set (like a map) and [valid] is satisfied 
+  by a set [s] under [k] only if all elements in [s] satisfy the validity property under [k]. 
 *)
 
-(** ** General leveled set interface *)
-Module Type IsLvlSetOTWLGenInterface (T : IsLvlOTWL) := (SetOTWithLeibnizInterface T) <+ IsLvl.
+(** *** Leveled Set Interface with ordered elements with leibniz equality *)
+Module Type IsLvlSetInterface (T : IsLvlOTWL) (Import St : SetOTWithLeibnizInterface T) 
+                                                                                  <: IsLvlOTWL.
 
-(** ** General leveled set interface without binders in its elements *)
-Module Type IsBdlLvlSetOTWLGenInterface (T : IsBdlLvlOTWL) 
-:= (SetOTWithLeibnizInterface T) <+ IsBdlLvl.
+  Include IsLvl St.
 
-(** ** Leveled set interface 
+  Definition t := t.
 
-  In addition to lemmas from [IsLvl], it is convenient to add lemmas that
-  describe the interaction between [shift], [valid] functions and classic functions like [add],[union],[singleton], etc.
-*)
-Module Type IsLvlSetOTWLInterface (T : IsLvlOTWL) <: IsLvlSetOTWLGenInterface T.
+  Definition eq := eq.
+  Definition eq_equiv := eq_equiv.
+  Definition eq_dec := eq_dec.
+  Definition eq_leibniz := eq_leibniz.
 
-  Include IsLvlSetOTWLGenInterface T.
+  Definition lt := lt.
+  Definition lt_strorder := lt_strorder.
+  Definition lt_compat := lt_compat.
 
-  (** *** Valid *)
+  Definition compare := compare.
+  Definition compare_spec := compare_spec.
+
+  (** **** Valid 
+    [valid] is opaque outside, consequently we gives an explicit unfold lemma.
+  *)
   Section valid.
 
     Variable lb : Lvl.t.
     Variable v : elt.
     Variable s s' : t.
 
-    (** [valid] is opaque outside, consequently we gives an explicit unfold lemma. *)
     Parameter valid_unfold : valid lb s <-> (For_all (T.valid lb) s).
     Parameter valid_add_spec : valid lb (add v s) -> T.valid lb v /\ valid lb s.
     Parameter valid_empty_spec : valid lb empty.
@@ -39,7 +49,7 @@ Module Type IsLvlSetOTWLInterface (T : IsLvlOTWL) <: IsLvlSetOTWLGenInterface T.
 
   End valid.
 
-  (** *** Shift *)
+  (** **** Shift *)
   Section shift.
 
     Variable lb k : Lvl.t.
@@ -67,64 +77,20 @@ Module Type IsLvlSetOTWLInterface (T : IsLvlOTWL) <: IsLvlSetOTWLGenInterface T.
 
   End shift.
 
-End IsLvlSetOTWLInterface.
+End IsLvlSetInterface.
 
-(** ** Set interface fully constrained with extra lemmas *)
-Module Type IsBdlLvlSetOTWLInterface (T : IsBdlLvlOTWL) 
-                                                <: IsBdlLvlSetOTWLGenInterface T.
+(** ---- *)
 
-  Include IsBdlLvlSetOTWLGenInterface T.
+(** *** Bindless Leveled Set Interface with ordered elements with leibniz equality *)
+Module Type IsBdlLvlSetInterface (T : IsLvlOTWL) (St : SetOTWithLeibnizInterface T) <: IsBdlLvlOTWL
+:= IsLvlSetInterface T St <+ IsBindlessLeveledEx.
 
-  (** *** Valid *)
-  Section valid.
 
-    Variable lb : Lvl.t.
-    Variable v : elt.
-    Variable s s' : t.
-    
-    Parameter valid_unfold : valid lb s <-> (For_all (T.valid lb) s).
-    Parameter valid_add_spec : valid lb (add v s) -> T.valid lb v /\ valid lb s.
-    Parameter valid_empty_spec : valid lb empty.
-    Parameter valid_union_spec : valid lb (union s s') <-> valid lb s /\ valid lb s'.
-    Parameter valid_singleton_spec : valid lb (singleton v) <-> T.valid lb v.
-    Parameter valid_in_spec : valid lb s -> In v s -> T.valid lb v.
+(** *** Leveled Set interface with boolean version of [valid] named [validb] *)
+Module Type IsLvlFullSetInterface (T : IsLvlFullOTWL) (St : SetOTWithLeibnizInterface T)
+:= (IsLvlSetInterface T St) <+ HasValidFull.
 
-  End valid.
 
-  (** *** Shift *)
-  Section shift.
-
-    Variable lb k : Lvl.t.
-    Variable v : elt.
-    Variable s s' : t.
-
-    Parameter shift_Empty_spec : Empty s -> shift lb k s = empty.
-    Parameter shift_empty_spec : shift lb k empty = empty.
-    Parameter shift_singleton_spec : shift lb k (singleton v) = singleton (T.shift lb k v).
-    Parameter shift_union_spec : shift lb k (union s s') = union (shift lb k s) (shift lb k s').
-    Parameter shift_inter_spec : shift lb k (inter s s') = inter (shift lb k s) (shift lb k s').
-    Parameter shift_diff_spec : shift lb k (diff s s') = (diff (shift lb k s) (shift lb k s')).
-
-    Parameter shift_add_notin_spec :
-      ~ In v s -> shift lb k (add v s) = add (T.shift lb k v) (shift lb k s).
-    Parameter shift_add_in_spec : In v s -> shift lb k (add v s) = (shift lb k s).
-    Parameter shift_add_spec : shift lb k (add v s) = add (T.shift lb k v) (shift lb k s).
-    Parameter shift_remove_spec : shift lb k (remove v s) = remove (T.shift lb k v)(shift lb k s).
-    
-    Parameter shift_in_spec : In v s <-> In (T.shift lb k v) (shift lb k s).
-    Parameter shift_in_e_spec :
-      In v (shift lb k s) -> 
-      exists v', v = (T.shift lb k v') /\ In (T.shift lb k v') (shift lb k s).
-    Parameter shift_notin_spec : ~ In v s <-> ~ In (T.shift lb k v) (shift lb k s).
-
-  End shift.
-
-End IsBdlLvlSetOTWLInterface.
-
-(** ** Set interface with minimal constraints, extra lemmas and [validb] *)
-Module Type IsLvlFullSetOTWLInterface (T : IsLvlFullOTWL) 
-:= (IsLvlSetOTWLInterface T) <+ HasValidFull.
-
-(** ** Set interface fully constrained with extra lemmas and [validb] *)
-Module Type IsBdlLvlFullSetOTWLInterface (T : IsBdlLvlFullOTWL) 
-:= (IsBdlLvlSetOTWLInterface T) <+ HasValidFull.
+(** *** Bindless Leveled Set interface with boolean version of [valid] named [validb] *)
+Module Type IsBdlLvlFullSetInterface (T : IsBdlLvlFullOTWL) (St : SetOTWithLeibnizInterface T)
+:= (IsBdlLvlSetInterface T St) <+ HasValidFull.
